add paco like new coinduction using approximation and scott continuous functions

fstar/RG.fst
@@ -1,7 +1,49 @@
 module RG
 
+open FStar.Monotonic.Pure
 module Map = FStar.Map
-module P = FStar.Preorder
+module U = Utils
 
-let st_pre (state:Type0) (rely guarantee:P.relation state) =
-  p:(state -> Type0){P.stable p rely}
+let rg_pre (state:Type0) (rely:U.preorder state) =
+  p:(state -> Type0){U.stable p rely}
+
+let rg_post (a:Type) (state:Type0)
+  (rely:U.preorder state) (pre:rg_pre state rely) =
+  state -> a -> rg_pre state rely
+
+
+type rg_repr (a:Type) (state:Type0) (rely guarantee:U.preorder state)
+  (pre:rg_pre state rely) (post:rg_post a state rely pre) =
+  s0:state -> Div (a & state)
+    (requires pre s0)
+    (ensures fun (x, s1) ->
+      post s0 x s1
+    )
+
+
+let rg_return (a:Type) (state:Type0)
+  (rely guarantee:U.preorder state) (x:a)
+  : rg_repr a state rely guarantee
+    (fun _ -> True) (fun s0 y s1 -> x == y /\ rely s0 s1)
+  = fun s0 -> (x, s0)
+
+let stabilize (a:Type) (p:U.predicate a) (r:U.preorder a) : 
+  p':U.predicate a{U.stable p r} =
+  admit()
+
+let rg_bind (a b:Type) (state:Type0)
+  (rely guarantee:U.preorder state)
+
+  (pre_f: rg_pre state rely)
+  (post_f:rg_post a state rely pre_f)
+
+  (pre_g:a -> rg_pre state rely)
+  (post_g:(x:a) -> rg_post b state rely (pre_g x))
+
+  (f:rg_repr a state rely guarantee pre_f post_f)
+  (g:(x:a) -> rg_repr b state rely guarantee (pre_g x) (post_g x))
+
+  : rg_repr b state rely guarantee
+    (fun s0 -> pre_f s0 /\ (forall x s1. post_f s0 x s1 ==> pre_g x s1))
+    (fun s0 y s2 -> exists x s1. post_f s0 x s1 /\ post_g x s1 y s2)
+  = fun s0 -> let (x, s1) = f s0 in g x s1
